Started with Ultimate SLH with Sebastian and Rob

UltimateSLH.v
@@ -1,4 +1,4 @@
-(** * SpecRelative: Relative Security Against Speculation Attacks*)
+(** * UltimateSLH: Relative Security Against Speculation Attacks*)
 
 (* TERSE: HIDEFROMHTML *)
 Set Warnings "-notation-overridden,-parsing,-deprecated-hint-without-locality".
@@ -22,13 +22,11 @@ Set Default Goal Selector "!".
     relative notion of security which intuitively ensures that the protected
     program does not leak more information speculatively than the original
     program leaks sequentially via the CT observations. One way to achieve this
-    protection is by transforming the program using standard Speculative Load
-    Hardening (SLH), instead of the selective variant from the previous chapter. *)
+    protection is by transforming the program using Ultimate Speculative Load
+    Hardening (USLH), instead of the selective variant from the previous chapter. *)
 
 (** We formalize this as a relative security property that doesn't label data at
-    all as public or secret. This seems to roughly correspond to the "weak
-    speculative non-interference" from the paper "Hardware-Software Contracts
-    for Secure Speculation" (IEEE SP 2021). *)
+    all as public or secret. *)
 
 Definition seq_obs_secure c st1 st2 ast1 ast2 : Prop :=
   forall stt1 stt2 astt1 astt2 os1 os2,
@@ -47,36 +45,75 @@ Definition relative_secure (trans : com -> com) (c:com) (st1 st2:state) : Prop :
     seq_obs_secure c st1 st2 ast1 ast2 ->
     spec_obs_secure (trans c) st1 st2 ast1 ast2.
 
-(** * Standard Speculative Load Hardening (SLH, not selective *)
+(** * Ultimate Speculative Load Hardening *)
 
-Definition AllPub : pub_vars := (_!-> true).
+(* HIDE: With BOr cand do [be || "b" <> 0], but whatever can also do it with BAnd
+Definition BOr b1 b2 := BNot (BAnd (BNot b1) (BNot b2)).
+Notation "x || y"  := (BOr x y) (in custom com at level 80, left associativity). *)
 
-Definition slh := sel_slh AllPub.
+Axiom MASK : nat.
 
-Definition ideal_eval_slh := ideal_eval AllPub.
+Fixpoint ultimate_slh (c:com) :=
+  (match c with
+  | <{{skip}}> => <{{skip}}>
+  | <{{x := e}}> => <{{x := e}}>
+  | <{{c1; c2}}> => <{{ ultimate_slh c1; ultimate_slh c2}}>
+  | <{{if be then c1 else c2 end}}> =>
+      <{{if be && "b" = 0 then "b" := (be ? "b" : 1); ultimate_slh c1
+                          else "b" := (be ? 1 : "b"); ultimate_slh c2 end}}>
+  | <{{while be do c end}}> =>
+      <{{while be && "b" = 0 do "b" := (be ? "b" : 1); ultimate_slh c end;
+         "b" := (be ? 1 : "b")}}>
+  | <{{x <- a[[i]]}}> =>
+    <{{x <- a[[("b" = 1) ? 0 : i]] }}>
+  | <{{a[i] <- e}}> => <{{a[("b" = 1) ? 0 : i] <- e}}>
+  end)%string.
 
-(* We can reuse the BCC proof for proving [relative_secure slh] *)
+Fixpoint observations (c:com) (ds:dirs) : obs :=
+  match c with
+  | <{{skip}}> => []
+  | <{{x := e}}> => []
+  | <{{c1; c2}}> => observations c2 ds ++ observations c1 ds
+  | <{{if be then c1 else c2 end}}> => observations c2 ds ++ [OBranch false]
+  | <{{while be do c end}}> => []
+  | <{{x <- a[[i]]}}> => [OARead a 0]
+  | <{{a[i] <- e}}> => [OAWrite a 0]
+  end.
 
-Lemma slh_bcc : forall c ds st ast (b: bool) st' ast' b' os,
+Lemma observations_fixed : forall c st ast ds stt astt os,
   unused "b" c ->
-  st "b" = (if b then 1 else 0) ->
-  <(st, ast, b, ds)> =[ slh c ]=> <(st', ast', b', os)> ->
-  AllPub |- <(st, ast, b, ds)> =[ c ]=> <("b" !-> st "b"; st', ast', b', os)>.
-Proof. intros; eapply sel_slh_ideal; eauto. Qed.
+  st "b" = 1 ->
+  <(st, ast, true, ds)> =[ ultimate_slh c ]=> <(stt, astt, true, os)> ->
+  os = observations c ds.
+Admitted.
 
-Conjecture same_final_b : forall P c s1 s2 as1 as2 b ds s1' s2' as1' as2' b1' b2' os1 os2,
-  P |- <( s1, as1, b, ds )> =[ c ]=> <( s1', as1', b1', os1 )> ->
-  P |- <( s2, as2, b, ds )> =[ c ]=> <( s2', as2', b2', os2 )> ->
-  b1' = b2'.
+Lemma gilles_lemma : forall c st1 st2 ast1 ast2 ds stt1 stt2 astt1 astt2 os1 os2,
+  unused "b" c ->
+  st1 "b" = 1 ->
+  st2 "b" = 1 ->
+  <(st1, ast1, true, ds)> =[ ultimate_slh c ]=> <(stt1, astt1, true, os1)> ->
+  <(st2, ast2, true, ds)> =[ ultimate_slh c ]=> <(stt2, astt2, true, os2)> ->
+  os1 = os2.
+Proof.
+  intros c st1 st2 ast1 ast2 ds stt1 stt2 astt1 astt2 os1 os2 Hunused Hb1 Hb2 H1 H2.
+  apply observations_fixed in H1; try auto.
+  apply observations_fixed in H2; try auto. congruence.
+Qed.
 
-Conjecture ideal_eval_no_spec : forall P c s ast ds s' ast' os,
-  P |- <( s, ast, false, ds )> =[ c ]=> <( s', ast', false, os )> ->
-  (forall d, In d ds -> d = DStep).
+(* TODO: this should be defined wrt a new ideal semantics for Ultimate SLH *)
+Definition ideal_spec_obs_secure c st1 st2 ast1 ast2 : Prop :=
+  forall ds stt1 stt2 astt1 astt2 bt1 bt2 os1 os2,
+    <(st1, ast1, false, ds)> =[ c ]=> <(stt1, astt1, bt1, os1)> ->
+    <(st2, ast2, false, ds)> =[ c ]=> <(stt2, astt2, bt2, os2)> ->
+    os1 = os2.
 
-Conjecture ideal_eval_no_spec_to_seq : forall P c s ast ds s' ast' os,
-  (forall d, In d ds -> d = DStep) ->
-  P |- <( s, ast, false, ds )> =[ c ]=> <( s', ast', false, os )> ->
-  <( s, ast )> =[ c ]=> <( s', ast', os )>.
+Lemma relative_noninterference : forall c st1 st2 ast1 ast2,
+  unused "b" c ->
+  st1 "b" = 1 ->
+  st2 "b" = 1 ->
+  seq_obs_secure c st1 st2 ast1 ast2 ->
+  ideal_spec_obs_secure c st1 st2 ast1 ast2.
+Admitted.
 
 Theorem relative_secure_slh :
   forall c st1 st2,
@@ -84,88 +121,5 @@ Theorem relative_secure_slh :
     unused "b" c ->
     st1 "b" = 0 ->
     st2 "b" = 0 ->
-    relative_secure slh c st1 st2.
-Proof.
-  unfold relative_secure, seq_obs_secure, spec_obs_secure.
-  intros c st1 st2 Hunused Hst1b Hst2b Hseq ds ast1 ast2 stt1 stt2 astt1 astt2 bt1 bt2 os1 os2 Hev1 Hev2.
-  apply slh_bcc in Hev1; try assumption.
-  apply slh_bcc in Hev2; try assumption.
-  eapply same_final_b in Hev1 as SameB; try eassumption. subst.
-  destruct bt1 eqn:Eqbt1.
-  - (* with speculation *)
-    destruct c as [| X e | c1 c2 | be ct cf | be cw | X a ie | a ie e ] eqn:Eqnc;
-    inversion Hev1; subst; clear Hev1; inversion Hev2; subst; clear Hev2;
-    simpl in *; eauto.
-    + (* Ideal_Seq *) admit.
-    + (* Ideal_If *) admit.
-    + (* Ideal If_F *) admit.
-    + (* Ideal_While *) admit.
-  - (* without speculation *)
-    pose proof (ideal_eval_no_spec _ _ _ _ _ _ _ _ Hev1) as NoSpec.
-    eapply ideal_eval_no_spec_to_seq in Hev1; try assumption.
-    eapply ideal_eval_no_spec_to_seq in Hev2; try assumption.
-    eauto.
-Admitted.
-
-Fixpoint sub_com (c1 c2 :com) :Prop :=
-  match c2 with 
-  | <{{ c21; c22 }}> => c1 = c2 \/ sub_com c1 c21 \/ sub_com c1 c22
-  | <{{ if be2 then ct2 else cf2 end }}> =>
-        c1 = c2 \/ sub_com c1 ct2 \/ sub_com c1 cf2
-  | <{{ while be2 do cw2 end }}> => c1 = c2 \/ sub_com c1 cw2
-  | _ => c1 = c2
-  end.
-
-Lemma sub_com_refl : forall c, sub_com c c.
-Proof. destruct c; simpl; auto. Qed.
-
-Lemma sub_com_seq_obs_secure : forall c1 c2 st1 st2 ast1 ast2,
-  spec_obs_secure c2 st1 st2 ast1 ast2 ->
-  sub_com c1 c2 ->
-  spec_obs_secure c1 st1 st2 ast1 ast2.
-Proof.
-Admitted.
-
-Fixpoint branch_on_bexp (be :bexp) (c :com) :Prop :=
-  match c with
-  | <{{ c1; c2 }}> =>  branch_on_bexp be c1 \/ branch_on_bexp be c2
-  | <{{ if be' then ct else cf end }}> => 
-        be = be' \/ branch_on_bexp be ct \/ branch_on_bexp be cf
-  | <{{ while be' do cw end }}> => be = be' \/ branch_on_bexp be cw
-  | _  => False
-  end.
-
-Definition branch_equiv (c :com) (st1 st2 :state) :Prop :=
-  forall be, branch_on_bexp be c -> beval st1 be = beval st2 be.
-
-Lemma branch_equiv_sub_com : forall c1 c2 st1 st2,
-  branch_equiv c2 st1 st2 ->
-  sub_com c1 c2 ->
-  branch_equiv c1 st1 st2.
-Admitted.
-
-Lemma seq_obs_secure_branch_equiv : forall c st1 st2 ast1 ast2,
-  seq_obs_secure c st1 st2 ast1 ast2 ->
-  branch_equiv c st1 st2.
-Proof.
-Admitted.
-
-Fixpoint access_on_index (ie :aexp) (c :com) :Prop :=
-  match c with
-  | <{{ c1; c2 }}> =>  access_on_index ie c1 \/ access_on_index ie c2
-  | <{{ if be then ct else cf end }}> => 
-        access_on_index ie ct \/ access_on_index ie cf
-  | <{{ while be do cw end }}> => access_on_index ie cw
-  | <{{ X <- A[[ie']] }}> => ie = ie'
-  | <{{ A[ie'] <- e}}> => ie = ie'
-  | _  => False
-  end.
-
-Definition index_equiv (c :com) (st1 st2 :state) :Prop :=
-  forall ie, access_on_index ie c -> aeval st1 ie = aeval st2 ie.
-
-Lemma seq_obs_secure_index_equiv : forall c st1 st2 ast1 ast2,
-  seq_obs_secure c st1 st2 ast1 ast2 ->
-  index_equiv c st1 st2.
-Proof.
-Admitted.
+    relative_secure ultimate_slh c st1 st2.
+Admitted. (* from relative noninterference + bcc *)
